current-formalism/Core/RobotInfo.v
@@ -1,18 +1,19 @@
 (**************************************************************************)
-(*   Mechanised Framework for Local Interactions & Distributed Algorithms *)
-(*   T. Balabonski, P. Courtieu, L. Rieg, X. Urbain                       *)
-(*   PACTOLE project                                                      *)
+(*  Mechanised Framework for Local Interactions & Distributed Algorithms  *)
+(*  T. Balabonski, P. Courtieu, L. Rieg, X. Urbain                        *)
+(*  PACTOLE project                                                       *)
 (*                                                                        *)
-(*   This file is distributed under the terms of the CeCILL-C licence     *)
+(*  This file is distributed under the terms of the CeCILL-C licence      *)
 (*                                                                        *)
 (**************************************************************************)
 
-(**  Mechanised Framework for Local Interactions & Distributed Algorithms   
-     T. Balabonski, P. Courtieu, L. Rieg, X. Urbain                         
+(** Mechanised Framework for Local Interactions & Distributed Algorithms    
                                                                             
-     PACTOLE project                                                        
+    T. Balabonski, P. Courtieu, L. Rieg, X. Urbain                          
                                                                             
-     This file is distributed under the terms of the CeCILL-C licence     *)
+    PACTOLE project                                                         
+                                                                            
+    This file is distributed under the terms of the CeCILL-C licence      *)
 
 
 Require Import Rbase.
@@ -36,7 +37,6 @@ Set Implicit Arguments.
 (** The minimum we ask for is the current location of the robot. *)
 Class IsLocation loc info `{EqDec info} `{EqDec loc} := {
   get_location : info -> loc;
-(*   update_location : loc -> info -> info; (* The [loc] argument is relative to the current location *) *)
   (** Lifting a change of frame to the location field *)
   app : (loc -> loc) -> info -> info;
   app_id : @equiv _ (fun_equiv _ _) (app id) id;
@@ -44,25 +44,13 @@ Class IsLocation loc info `{EqDec info} `{EqDec loc} := {
   get_location_app : forall f state, get_location (app f state) == f (get_location state);
   (** Compatibility properties *)
   get_location_compat :> Proper (equiv ==> equiv) get_location;
-(*   update_location_compat :> Proper (equiv ==> equiv ==> equiv) update_location; *)
   app_compat :> Proper ((equiv ==> equiv) ==> equiv ==> equiv) app }.
 
 Arguments IsLocation loc info {_} {_} {_} {_}.
 
-
-(** Same class but different name. *)
-Class IsTarget loc info `{IsLocation loc info} := {
-  get_target : info -> loc;
-(*   update_target : loc -> info -> info; *)
-  get_target_app : forall f state, get_target (app f state) == f (get_target state);
-  (** Compatibility properties *)
-  get_target_compat :> Proper (equiv ==> equiv) get_target }.
-(*   update_target_compat :> Proper (equiv ==> equiv ==> equiv) update_target }. *)
-
-Arguments IsTarget loc info {_} {_} {_} {_} {_}.
-
 (* TODO: Define the disjoint union of such projections to ensure their independence. *)
 
+(** A basic state containing only the current location. *)
 Definition OnlyLocation loc `{EqDec loc} : IsLocation loc loc := {|
   get_location := id;
   app := id;
@@ -70,13 +58,8 @@ Definition OnlyLocation loc `{EqDec loc} : IsLocation loc loc := {|
   app_compose := ltac:(reflexivity);
   get_location_app := ltac:(reflexivity) |}.
 
-
-Section AddInfo.
-
-Variable T : Type.
-Context `{EqDec T}.
-
-Instance AddInfo loc info `(IsLocation loc info) : IsLocation loc (info * T) := {|
+(** Adding information that is not affected by frame change. *)
+Instance AddInfo T loc info `{EqDec T} `(IsLocation loc info) : IsLocation loc (info * T) := {|
   get_location := fun x => get_location (fst x);
   app := fun f x => (app f (fst x), snd x) |}.
 Proof.
@@ -87,9 +70,7 @@ Proof.
 + intros f g Hfg [] [] []. simpl. repeat split; trivial; []. now apply app_compat.
 Defined.
 
-End AddInfo.
-
-
+(** Adding a location-typed field that is affected by frame change. *)
 Instance AddLocation loc info `(IsLocation loc info) : IsLocation loc (info * loc) := {|
   get_location := fun x => get_location (fst x);
   app := fun f x => (app f (fst x), f (snd x)) |}.
